% Exercise 1.1.2

\begin{proof}
    \begin{itemize}
        \item[($\Rightarrow$)]
            First, suppose we have
            \[
                \frac{\lvert \text{fl}(x) - x \rvert}{\lvert x \rvert}
                \leq \frac{2^{n-d-1}}{2^n} \leq \frac{1}{2}\epsilon_{\text{mach}},
            \]
            so that
            \begin{equation*}
                \begin{split}
                    \lvert \text{fl}(x) - x \rvert &\leq \frac{\lvert x \rvert}{2}
                    \epsilon_{\text{mach}} \\
                    \Leftrightarrow -\frac{\lvert x \rvert}{2}\epsilon_{\text{mach}}
                    \leq \text{fl}(x) - x &\leq \frac{\lvert x \rvert}{2}
                    \epsilon_{\text{mach}} \\
                    \Leftrightarrow x - \frac{\lvert x \rvert}{2}\epsilon_{\text{mach}}
                    \leq \text{fl}(x) &\leq x + \frac{\lvert x \rvert}{2}
                    \epsilon_{\text{mach}} \\
                \end{split}
            \end{equation*}
            for
            \[
                \lvert \epsilon \rvert \leq \frac{1}{2}\epsilon_{\text{mach}}.
            \]
        \item[($\Leftarrow$)]
            Now, suppose that
            \[
                \text{fl}(x) = x(1 + \epsilon) \quad \text{for some} \quad 
                \lvert \epsilon \rvert \leq \frac{1}{2}\epsilon_{\text{mach}},
            \]
            so that
            \begin{equation*}
                \begin{split}
                    \text{fl}(x) - x &= \epsilon x\\
                    \Leftrightarrow \lvert \text{fl}(x) - x \rvert 
                                     &= \lvert \epsilon x \rvert \\
                    \Leftrightarrow \frac{\lvert \text{fl}(x) - x\rvert}{\lvert x \rvert}
                                     &= \lvert \epsilon \rvert \\
                                     &\leq \frac{1}{2}\epsilon_{\text{mach}}.
                \end{split} 
            \end{equation*}
    \end{itemize}
\end{proof}
